Pbasic.v
@@ -1785,7 +1785,7 @@ apply/existsP; exists i1; apply/existsP; exists j1.
 by apply/and5P; split; rewrite // !cell_lor ?(j1_gt2, Hc1, Hc2, Hc3, Hc4).
 Qed.
 
-Definition wf w b := [/\ wf_state (w lor b), ~~cwin w & ~~ cwin b].
+Definition wf_pos w b := [/\ wf_state (w lor b), ~~cwin w & ~~ cwin b].
 
 Definition nlhash := to_nat lhash.
 
