Pmain.v
@@ -33,7 +33,7 @@ Definition eh1 := hput ew1 eb1 10000000 win 0 (make_hash tt).
 
 Lemma valid_eh1 : valid_htable eh1.
 Proof.
-have /wfb_correct[H1 H2] : wfb ew1 eb1 by [].
+have /wf_posb_correct[H1 H2] : wf_posb ew1 eb1 by [].
 apply: valid_has_table_valid_hput => //; first by case: H1.
   rewrite -eval_ev1E.
   by exact: (topeval_correct (refl_equal true : wfb ew1 eb1 = _ )).
@@ -44,7 +44,7 @@ Definition eh2 := hput ew2 eb2 10000000 win 0 eh1.
 
 Lemma valid_eh2 : valid_htable eh2.
 Proof.
-have /wfb_correct[H1 H2] : wfb ew2 eb2 by [].
+have /wf_posb_correct[H1 H2] : wf_posb ew2 eb2 by [].
 apply: valid_has_table_valid_hput => //; first by case: H1.
   rewrite -eval_ev2E.
   by exact: (topeval_correct (refl_equal true : wfb ew2 eb2 = _ )).
@@ -55,7 +55,7 @@ Definition eh3 := hput ew3 eb3 10000000 win 0 eh2.
 
 Lemma valid_eh3 : valid_htable eh3.
 Proof.
-have /wfb_correct[H1 H2] : wfb ew3 eb3 by [].
+have /wf_posb_correct[H1 H2] : wf_posb ew3 eb3 by [].
 apply: valid_has_table_valid_hput => //; first by case: H1.
   rewrite -eval_ev3E.
   by exact: (topeval_correct (refl_equal true : wfb ew3 eb3 = _ )).
@@ -66,7 +66,7 @@ Definition eh4 := hput ew4 eb4 10000000 win 0 eh3.
 
 Lemma valid_eh4 : valid_htable eh4.
 Proof.
-have /wfb_correct[H1 H2] : wfb ew4 eb4 by [].
+have /wf_posb_correct[H1 H2] : wf_posb ew4 eb4 by [].
 apply: valid_has_table_valid_hput => //; first by case: H1.
   rewrite -eval_ev4E.
   by exact: (topeval_correct (refl_equal true : wfb ew4 eb4 = _ )).
@@ -83,5 +83,3 @@ suff <- : htop_eval empty_state empty_state eh4 = win.
 vm_cast_no_check (refl_equal win).
 Qed.
 
-Print eval.
-Print eval_aux.
